
\documentclass[11pt]{article}
\hfuzz 18pt

\usepackage{amsmath}
\usepackage{amssymb}
\usepackage{amsfonts}
\usepackage{xcolor}
\usepackage{bussproofs}
\EnableBpAbbreviations
\usepackage[a4paper, total={6in, 8in}]{geometry}

\newcommand{\B}{\mathbb{B}}
\newcommand{\N}{\texttt{Nat}}
\newcommand{\x}{\times}
\newcommand{\T}{\texttt{true}}
\newcommand{\U}{\texttt{unify}}
\newcommand{\rarr}{\rightarrow}
\renewcommand{\r}[1]{\texttt{right}(#1)}
\renewcommand{\l}[1]{\texttt{left}(#1)}

\title{Assignment 1 \\ Types}
\author{Sam Barrett, 1803086}
\begin{document}
\maketitle

\begin{enumerate}
	\item
	      \begin{multline*}
		      M ::= \lambda x.M | M M | \texttt{true} | \texttt{false} | \texttt{if } M \texttt{ then } M \texttt{ else } M|  \\
		      \langle M,M \rangle | \texttt{spread}(M,M) | \texttt{left}(M) | \texttt{right}(M)
	      \end{multline*}
	      \begin{flalign*}
		      T ::= \B | T \rarr T | T \x T | T + T
	      \end{flalign*}

	      \begin{enumerate}
		      \item Extend call-by-value small-step operational semantics of the Curry-style Simply Typed $\lambda$-Calculus

		            Values, $ V ::= \lambda x:T.M | \texttt{true} | \texttt{false} | \langle M,M \rangle | \l{M} | \r{M} $
		            Evaluation Contexts

		            \begin{multline*}
			            C::= \bullet | C M | V C | \texttt{if } C \texttt{ then } M \texttt{ else } M | \texttt{spread}(C,M) | \texttt{case}(C,M,M)
		            \end{multline*}

		            Rules:

		            \begin{prooftree}
			            \AxiomC{}
			            \RightLabel{$\beta$}
			            \UnaryInfC{$ (\lambda x:T.M)V \rarr_v M[x\backslash V] $}
		            \end{prooftree}

		            \begin{prooftree}
			            \AXC{}
			            \RightLabel{ITET}
			            \UIC{$ \texttt{if true then } M \texttt{ else } N \rarr_v M $}
		            \end{prooftree}

		            \begin{prooftree}
			            \AXC{}
			            \RL{ITEF}
			            \UIC{ $\texttt{if false then } M \texttt{ else } N \rarr_v N$}
		            \end{prooftree}

		            \begin{prooftree}
			            \AXC{$M \rarr_v N$}
			            \RL{$ \texttt{CTX}_C$}
			            \UIC{$C[M] \rarr_v C[N]$}
		            \end{prooftree}

		            \begin{prooftree}
			            \AXC{$M \rarr_v \langle P,Q \rangle$}
			            \RL{SP}
			            \UIC{ $\texttt{spread}(M,N) \rarr_v NPQ $}
		            \end{prooftree}

		            \begin{prooftree}
			            \AXC{$M \rarr_v \texttt{left}(N)$}
			            \RL{CL}
			            \UIC{ $ \texttt{case}(M,P,Q) \rarr_v NP$}
		            \end{prooftree}

		            \begin{prooftree}
			            \AXC{$M \rarr_v \texttt{right}(N)$}
			            \RL{CR}
			            \UIC{ $ \texttt{case}(M,P,Q) \rarr_v NQ$}
		            \end{prooftree}

		      \item
		            Prove:

			    \textbf{Note: unless stated otherwise $\Pi_{n-1}$ stands for the RHS of the bottom of the previous proof tree}

		            \begin{multline*}
			            \texttt{spread}(( \lambda x. \langle x,x \rangle ) \texttt{true}, \lambda y. \lambda z. \texttt{if } y \texttt{ then } \texttt{left}(z) \texttt{ else } \texttt{right}(z))  \\
			            \rarr_v^* \texttt{left(true)}
		            \end{multline*}

		            \begin{prooftree}
			            \AXC{$ \langle \texttt{true,true} \rangle$}
			            \RL{ $ \beta $ }
				    \UIC{ $ (\lambda x. \langle x,x \rangle ) \texttt{true}$}
			            \RL{ $ \texttt{spread}(\bullet,M)$ \;\;\;\; (1)}
			            \UIC{$\Pi$}
		            \end{prooftree}

		            Where $\Pi$ is defined as:
		            \begin{multline*}
			            \texttt{spread}(( \lambda x. \langle x,x \rangle ) \texttt{true},
			            \lambda y. \lambda z. \texttt{if } y \texttt{ then } \texttt{left}(z) \texttt{ else } \texttt{right}(z)) \\
			            \rarr_v \texttt{spread}( \langle \texttt{true,true} \rangle ,
			            \texttt{if } y \texttt{ then } \texttt{left}(z) \texttt{ else } \texttt{right}(z))
		            \end{multline*}


		            \begin{prooftree}
			            \AXC{}
			            \RL{SP \: \: \: (2)}
			            \UIC{ $\Pi_1 \rarr_v ( \lambda y. \lambda z. \texttt{if } y \texttt{ then } \l{z} \texttt{ else } \r{z}) \texttt{true true} $}
		            \end{prooftree}

		            \begin{prooftree}
			            \AXC{}
			            \RL{$\beta$ \;\;\; (3)}
				    \UIC{ $ \Pi_2 \rarr_v (\lambda z. \texttt{if true}  \texttt{ then } \l{z} \texttt{ else } \r{z}) \T $}
		            \end{prooftree}

		            \begin{prooftree}
			            \AXC{}
			            \RL{$\beta$ \;\;\; (4)}
			            \UIC{$ \Pi_3 \rarr_v \texttt{if } \texttt{true} \texttt{ then } \l{ \texttt{true}} \texttt{ else } \r{ \texttt{true}}$}
		            \end{prooftree}

		            \begin{prooftree}
			            \AXC{}
			            \RL{ITET \;\;\; (5)}
			            \UIC{ $ \Pi_4 \rarr_v \l{ \texttt{true}}$}
		            \end{prooftree}


		      \item
		            Typing Rules:

		            \begin{prooftree}
			            \AXC{}
			            \RL{VAR}
			            \UIC{ $ \Gamma , x:T \vdash x:T $}
		            \end{prooftree}

		            \begin{prooftree}
			            \AXC{$ \Gamma, x:T \vdash M:U$}
			            \RL{ABS}
			            \UIC{ $ \Gamma \vdash \lambda x:T.M:T \rarr U $}
		            \end{prooftree}

		            \begin{prooftree}
			            \AXC{ $\Gamma \vdash M:T \rarr U$}
			            \AXC{$\Gamma \vdash N:T$}
			            \RL{APP}
			            \BIC{ $ \Gamma \vdash MN :U $}
		            \end{prooftree}

		            \begin{prooftree}
			            \AXC{}
			            \RL{T}
			            \UIC{ $ \Gamma \vdash \texttt{true} : \B$}
		            \end{prooftree}

		            \begin{prooftree}
			            \AXC{}
			            \RL{F}
			            \UIC{ $\Gamma \vdash \texttt{false}: \B$}
		            \end{prooftree}

		            \begin{prooftree}
			            \AXC{$ \Gamma \vdash M: \B$}
			            \AXC{$ \Gamma \vdash N:T$}
			            \AXC{$ \Gamma \vdash P:T$}
			            \RL{ITE}
			            \TIC{$ \Gamma \vdash \texttt{if } M \texttt{ then } N \texttt{ else } P :T$}
		            \end{prooftree}

		            \begin{prooftree}
			            \AXC{$ \Gamma \vdash M:T$}
			            \AXC{$ \Gamma \vdash M:U$}
			            \RL{PAIR}
			            \BIC{$ \Gamma \vdash \langle M,N \rangle : T \x U $}
		            \end{prooftree}

		            \begin{prooftree}
			            \AXC{$ \Gamma \vdash M:T\x U$}
			            \AXC{$ \Gamma \vdash N:T \rarr U \rarr Z$}
			            \RL{SP}
			            \BIC{$ \Gamma \vdash \texttt{spread}(M,N):Z$}
		            \end{prooftree}

		            \begin{prooftree}
			            \AXC{$ \Gamma \vdash M:T$}
			            \RL{L}
			            \UIC{$ \Gamma \vdash \l{M} : T + U $}
		            \end{prooftree}

		            \begin{prooftree}
			            \AXC{$ \Gamma \vdash M:U$}
			            \RL{R}
			            \UIC{$ \Gamma \vdash \r{M} : T + U $}
		            \end{prooftree}

		            \begin{prooftree}
			            \AXC{$ \Gamma \vdash M:T$}
			            \AXC{$ \Gamma \vdash P:T\rarr Z$}
			            \RL{CASEL}
			            \BIC{$ \Gamma \vdash \texttt{case}( \l{M},P,Q): Z$}
		            \end{prooftree}

		            \begin{prooftree}
			            \AXC{$ \Gamma \vdash M:U$}
			            \AXC{$ \Gamma \vdash Q:U\rarr Z$}
			            \RL{CASER}
			            \BIC{$ \Gamma \vdash \texttt{case}(\r{M},P,Q):Z$}
		            \end{prooftree}

		      \item
		            Prove:
		            $$
			            \texttt{spread}(( \lambda x. \langle x,x \rangle ) \texttt{true}, \lambda y. \lambda z. \texttt{if } y \texttt{ then } \l{z} \texttt{ else } \r{z})
		            $$ has type $\B + \B$

		            \begin{prooftree}
			            \AXC{}
			            \RL{T}
			            \UIC{$ \texttt{true}: \B$}
			            \RL{L}
			            \UIC{$\l{ \texttt{true}} : \B + U$}
		            \end{prooftree}

		            Where $U$ is of \textbf{any} type, $\therefore$ we can say $U \mapsto \B$ giving us $\l{ \texttt{true}} : \B + \B$

	      \end{enumerate}

	\item
	      Is:

	      \[
		      ( \lambda x. \lambda y. ((xy)(x \texttt{true})
	      \]

	      typeable within the Simply Typed $\lambda$-Calculus?


	      \underline{Wand's Algorithm:}

	      \textbf{Note: where '$C=C$', $C$ has not changed since the previous line}

	      \begin{align}
		      C = \emptyset, G = { \langle \cdot ; M_0 ; \alpha_0 \rangle }
	      \end{align}
	      \begin{align}
		      C = \{ \alpha_0 = \alpha_1 \rarr \alpha_2 \}, G = { \langle x: \alpha_1; \lambda y. ((xy)(x \texttt{true})); \alpha_2 \rangle  }
	      \end{align}
	      \begin{align}
		      C = \{ \alpha_0 = \alpha_1 \rarr \alpha_2, \alpha_2 = \alpha_3 \rarr \alpha_4 \}, G = { \langle x: \alpha_1, y: \alpha_3 ; (xy)(x \T); \alpha_4 \rangle  }
	      \end{align}
	      \begin{multline}
		      C = C, G = \{ \langle x: \alpha_1, y: \alpha_3 ; xy ; \alpha_5 \rarr \alpha_4 \rangle, \langle x: \alpha_1, y:\alpha_3 ; x\T; \alpha_5 \rangle   \}
	      \end{multline}
	      \begin{multline}
		      C = C, \\
		      G = \{ \langle x: \alpha_1, y:\alpha_3 ; x ; \alpha_6 \rarr \alpha_5\rarr \alpha_4  \rangle , \langle x: \alpha_1, y:\alpha_3 ; y ; \alpha_6  \rangle , \langle x: \alpha_1, y:\alpha_3 ; x\T; \alpha_5  \rangle  \} 
	      \end{multline}
	      \begin{multline}
		      C = C, G = \{ \langle x: \alpha_1, y:\alpha_3 ; x ; \alpha_6 \rarr \alpha_5\rarr \alpha_4  \rangle , \langle x: \alpha_1, y:\alpha_3 ; y ; \alpha_6 \rangle,\\ \langle  x: \alpha_1, y:\alpha_3 ; x ; \alpha_7 \rarr \alpha_5  \rangle, \langle x: \alpha_1, y:\alpha_3 ; \T ; \alpha_7 \rangle \}                                                      
	      \end{multline}
	      \begin{multline}
		      C = \{ \alpha_0 = \alpha_1 \rarr \alpha_2, \alpha_2 = \alpha_3 \rarr \alpha_4, \alpha_6 \rarr \alpha_5 \rarr \alpha_4 = \alpha_1 \},   \\ 
		      G = \{ \langle x: \alpha_1, y:\alpha_3 ; y ; \alpha_6 \rangle, \langle  x: \alpha_1, y:\alpha_3 ; x ; \alpha_7 \rarr \alpha_5  \rangle, \langle x: \alpha_1, y:\alpha_3 ; \T ; \alpha_7 \rangle \}  
	      \end{multline}
	      \begin{multline}
		      C = \{  \alpha_0 = \alpha_1 \rarr \alpha_2, \alpha_2 = \alpha_3 \rarr \alpha_4, \alpha_6 \rarr \alpha_5 \rarr \alpha_4 = \alpha_1, \alpha_6 = \alpha_3 \},                                                                  \\ 
		      G = \{  \langle  x: \alpha_1, y:\alpha_3 ; x ; \alpha_7 \rarr \alpha_5  \rangle, \langle x: \alpha_1, y:\alpha_3 ; \T ; \alpha_7 \rangle \}
	      \end{multline}
	      \begin{multline}
		      C = \{ \alpha_0 = \alpha_1 \rarr \alpha_2, \alpha_2 = \alpha_3 \rarr \alpha_4, \alpha_6 \rarr \alpha_5 \rarr \alpha_4 = \alpha_1, \alpha_6 = \alpha_3, \alpha_7 \rarr \alpha_5 = \alpha_1 \},                               \\
		      G = \{ \langle x: \alpha_1, y:\alpha_3 ; \T ; \alpha_7 \rangle \}
	      \end{multline}
	      \begin{multline}
		      C = \{ \alpha_0 = \alpha_1 \rarr \alpha_2, \alpha_2 = \alpha_3 \rarr \alpha_4, \\
		      \alpha_6 \rarr \alpha_5 \rarr \alpha_4 = \alpha_1, \alpha_6 = \alpha_3, \alpha_7 \rarr \alpha_5 = \alpha_1, \alpha_7 = \B \},                \\ 
		      G = \emptyset
	      \end{multline}

	

	\underline{Robinson's Algorithm:}
	
	\begin{multline}
		\U( \{ \alpha_0 = \alpha_1 \rarr \alpha_2, \alpha_2 = \alpha_3 \rarr \alpha_4, \alpha_6 \rarr \alpha_5 \rarr \alpha_4 = \alpha_1, \\ \alpha_6 = \alpha_3, \alpha_7 \rarr \alpha_5 = \alpha_1, \alpha_7 = \B \}) 
	\end{multline}
	\begin{multline}
		\U( \{ \alpha_2 = \alpha_3 \rarr \alpha_4, \alpha_6 \rarr \alpha_5 \rarr \alpha_4 = \alpha_1, \alpha_6 = \alpha_3, \alpha_7 \rarr \alpha_5 = \alpha_1, \alpha_7 = \B \}  ) \circ \\ ( \alpha_0 \mapsto \alpha_1 \rarr \alpha_2 )
	\end{multline}

	\begin{multline}
		\U( \{ \alpha_6 \rarr \alpha_6 \rarr \alpha_4 = \alpha_1, \alpha_6 = \alpha_3, \alpha_7 \rarr \alpha_5 = \alpha_1, \alpha_7 = \B \} )\circ \\ ( \alpha_2 \mapsto \alpha_3 \rarr \alpha_4) \circ ( \alpha_0 \mapsto \alpha_1 \rarr \alpha_2) 
	\end{multline}

	\begin{multline}
		\U( \{ \alpha_6 = \alpha_3, \alpha_7 \rarr \alpha_4 = \alpha_6 \rarr \alpha_5 \rarr \alpha_5, \alpha_7 = \B \} ) \circ \\ ( \alpha_1 \mapsto \alpha_6 \rarr \alpha_5 \rarr \alpha_4) \circ ( \alpha_2 \mapsto \alpha_3 \rarr \alpha_4) \circ ( \alpha_0 \mapsto \alpha_1 \rarr \alpha_2) 
	\end{multline}
	\begin{multline}
		\U( \{ \alpha_7 \rarr \alpha_5 = \alpha_3 \rarr \alpha_5 \rarr \alpha_4, \alpha_7 = \B \}  ) \circ \\
		( \alpha_6 \mapsto \alpha_3) \circ  ( \alpha_1 \mapsto \alpha_6 \rarr \alpha_5 \rarr \alpha_4) \circ ( \alpha_2 \mapsto \alpha_3 \rarr \alpha_4) \circ ( \alpha_0 \mapsto \alpha_1 \rarr \alpha_2) 
	\end{multline}
	\begin{multline}
		\U( \{ \alpha_7 = \B, \alpha_7 = \alpha_3 \rarr \alpha_5, \alpha_5 = \alpha_4 \} ) \circ \\ 
			( \alpha_6 \mapsto \alpha_3) \circ  ( \alpha_1 \mapsto \alpha_6 \rarr \alpha_5 \rarr \alpha_4) \circ ( \alpha_2 \mapsto \alpha_3 \rarr \alpha_4) \circ ( \alpha_0 \mapsto \alpha_1 \rarr \alpha_2) 
	\end{multline}
	\begin{multline}
		\U( \{ \B = \alpha_3 \rarr \alpha_5, \alpha_5 = \alpha_4 \} ) \circ ( \alpha_7 \mapsto \B) \circ ( \alpha_6 \mapsto \alpha_3) \\
			\circ  ( \alpha_1 \mapsto \alpha_6 \rarr \alpha_5 \rarr \alpha_4) \circ ( \alpha_2 \mapsto \alpha_3 \rarr \alpha_4) \circ ( \alpha_0 \mapsto \alpha_1 \rarr \alpha_2) 
	\end{multline}

	\color{red}
	ERROR: Cannot have constraint of the form $\B = T_1 \rarr T_2$ ! Therefore expression is not typable 

	\color{black}
\item 
	\begin{enumerate}

		\item 

			Define a successor function $ \texttt{Succ}: \N \rarr \N$ that takes a number and computes its successor.

			\begin{equation*}
				\texttt{Succ} = \lambda a:\N. \lambda \alpha'. \lambda f: \alpha' \rarr \alpha' . \lambda x: \alpha' . f(a \{ \alpha' \} fx)
			\end{equation*}

			And prove that it is well-typed: 

			\small\begin{prooftree}
				\AXC{}
				\RL{VAR}
				\UIC{$ \Gamma \vdash f: \alpha' \rarr \alpha' $}
				\AXC{$\Pi_1$}
				\RL{APP}
				\BIC{ $ \Gamma, x: \alpha'  \vdash f(a \{ \alpha'  \} fx) : \alpha' $}
				\RL{ABS}
				\UIC{$ \Gamma, f: \alpha' \rarr \alpha' \vdash \lambda x: \alpha' . f(a \{ \alpha'  \} fx) : \alpha' \rarr \alpha' $}
				\RL{ABS}
				\UIC{ $ \Gamma \vdash \lambda f: \alpha' \rarr \alpha' . \lambda x: \alpha' . f(a \{ \alpha'  \} fx) : ( \alpha' \rarr \alpha' ) \rarr \alpha' \rarr \alpha'$}
				\RL{TABS}
			\UIC{$ a: \N \vdash \lambda \alpha'. \lambda f: \alpha' \rarr \alpha'. \lambda x: \alpha' . f(a \{ \alpha'  \} fx) : \forall \alpha' . ( \alpha' \rarr \alpha' ) \rarr \alpha'  \rarr \alpha'$}
				\RL{ABS}
				\UIC{ $\cdot \vdash \lambda a: \N . \lambda \alpha'. \lambda f: \alpha' \rarr \alpha', \lambda x: \alpha'. f(a \{ \alpha'  \} fx): \N \rarr \N $}
			\end{prooftree}

			Where $\Pi_1$ is: 

			\small\begin{prooftree}
				\AXC{}
				\RL{VAR}
				\UIC{$ \Gamma \vdash f: \alpha' \rarr \alpha' $}
				\AXC{$ \Gamma \vdash a : \forall \alpha . ( \alpha \rarr \alpha ) \rarr \alpha \rarr \alpha$ }
				\RL{TAPP}
				\UIC{$ \Gamma \vdash a \{ \alpha'  \} : ( \alpha' \rarr \alpha' ) \rarr \alpha' \rarr \alpha' $}
				\RL{APP}
				\BIC{ $ \Gamma \vdash a \{ \alpha'  \} f: \alpha' \rarr \alpha' $}
				\AXC{}
				\RL{VAR}
				\UIC{$ \Gamma \vdash x: \alpha' $}
				\RL{APP}
				\BIC{$ \Gamma \vdash (a \{ \alpha' \} f)x : \alpha' $}
			\end{prooftree}

		\item 
			Define an addition function $ \texttt{Add} : \N \rarr \N \rarr \N$ that makes use of the successor function $ \texttt{Succ}$

			\begin{equation*}
				\texttt{Add} = \lambda a: \N. \lambda b: \N. a \{ \N \} \texttt{Succ} b
			\end{equation*}

			\begin{prooftree}
				\AXC{$ \Pi $}
				\AXC{ Proved above }
				\UIC{$ \Gamma \vdash \texttt{Succ} : \N \rarr \N $}

				\RL{APP}
				\BIC{$ \Gamma \vdash a \{ \N \} \texttt{Succ} : \N \rarr \N$}

				\AXC{}
				\RL{VAR}
				\UIC{$ \Gamma \vdash b: \N$}

				\RL{APP}
				\BIC{$ a:\N, b:\N \vdash a \{ \N \} \texttt{Succ}b : \N$}

				\RL{ABS}
				\UIC{$ a:\N \vdash  \lambda b:\N. a \{ \N \} \texttt{Succ}b : \N \rarr \N$}

				\RL{ABS}
				\UIC{ $ \cdot \vdash \lambda a: \N. \lambda b:\N. a \{ \N \} \texttt{Succ}b : \N \rarr \N \rarr \N $}
				
			
			\end{prooftree}

			$\Pi$ :
			\begin{prooftree}
				\AXC{}
				\RL{VAR}
				\UIC{ $ \Gamma \vdash a : \forall \alpha. ( \alpha \rarr \alpha ) \rarr \alpha \rarr \alpha $}
				\RL{TAPP}
				\UIC{$ \Gamma \vdash a \{ \N \} : ( \N \rarr \N ) \rarr \N \rarr \N $}
			\end{prooftree}
	\end{enumerate}
\end{enumerate}

\end{document}
